added some proofs

FY/Examples.v
@@ -4,15 +4,62 @@ Import ListNotations.
 From FY Require Export Utils.
 From FY Require Export Syntax.
 From FY Require Export Semantics.
-
+From FY Require Export Assertion.
 
 Definition X : string := "X".
+Definition Y : string := "Y".
+
+Check <{ X + (3 % nat) }>.
+
+Example aexp1 :
+    aeval (X !-> 5%nat; Y !-> 3%nat ; _ !-> 0%nat) <{ X + (3 % nat) - Y }> = 5%nat.
+Proof. reflexivity. Qed.
+
+Example bexp1 :
+    beval (X !-> 5%nat; Y !-> 3%nat ; _ !-> 0%nat) <{ Y <= X }> = true.
+Proof. reflexivity. Qed.
+
+Check H.
+
+Example state1:
+  ApplyOneQubitGate 0%nat 0%nat H = H.
+Proof.
+  reflexivity.
+Qed.
+
+Example state2:
+  ApplyOneQubitGate 0%nat 0%nat CNOT = CNOT.
+Proof.
+  reflexivity.
+Qed.
+
+Example state3:
+  ApplyOneQubitGate 1%nat 0%nat H = H.
+Proof.
+Admitted.
+
+Definition assert : Assertion 2 := fun (tmn: total_map nat) => pair (le (tmn X) 2%nat) H.
+
+Example satisfied: fst (assert (X !-> 0%nat; _ !-> 1%nat)).
+Proof.
+  simpl.
+  auto.
+Qed.
 
 Definition Prog1 : com :=
   <{ q 0 := 0;
      q 0 *= GH;
-     X :=measQ 0%nat }>.
+     X :=measQ 0 }>.
 Print Prog1.
+
+Theorem state_eval_1: ceval Prog1 [((_ !-> 0%nat), I 2)] [((X !-> 0%nat ; _ !-> 1%nat), H) ; ((X !-> 1%nat; _ !-> 1%nat), H)].
+Proof.
+  eapply E_Seq.
+  apply E_Init.
+  eapply E_Seq.
+  apply E_AppOne.
+Admitted.
+
 
 (* ENONTRA BOM EXEMPLOS PARA APRESENTAÇÃO*)
 (* () -> ∣0⟩⟨0∣ . I *)
@@ -27,9 +74,9 @@ Definition Prog2 : com :=
   <{ q 0 := 0;
      q 0 *= GH;
      X :=measQ 0%nat;
-     if BEq X 2%nat then
+     if false then
         q 0 *= GZ
-    else
+     else
         skip
     end }>.
 Print Prog2.
@@ -38,30 +85,23 @@ Definition Prog3 : com :=
   <{ q 0 := 0;
      q 0 *= GH }>.
 
+Theorem state_eval_3: ceval Prog3 [((_ !-> 0%nat), I 2)] [((_ !-> 0%nat), H ⊗ ∣0⟩⟨0∣ ⊗ H†)].
+Proof.
+Admitted.
 
 Definition Prog4 : com :=
   <{ q 0%nat := 0 }>.
 
-Definition zero := 0%nat.
-
 Definition Prog5 : com :=
-  <{ X :=c APlus 0%nat 1%nat }>.
+  <{ X :=c (2 % nat) }>.
 
-Theorem state_eval_1: ceval Prog1 [((_ !-> 0%nat), I 2)] [((X !-> 0%nat ; _ !-> 1%nat), H) ; ((X !-> 1%nat; _ !-> 1%nat), H)].
+Theorem state_eval_5: ceval Prog5 [((_ !-> 0%nat), I 2%nat)] [((X !-> 2%nat; _ !-> 0%nat), I 2%nat)].
 Proof.
-  eapply E_Seq.
-  apply E_Init.
-  eapply E_Seq.
-  apply E_App.
-  apply E_Meas.
-  apply E_Seq with [((X !-> 0%nat ; _ !-> 0%nat), H) ; ((X !-> 1%nat; _ !-> 0%nat), H)].
-
-Admitted.
+  eapply E_Ass.
+Qed.
 
 
-Theorem state_eval_3: ceval <{ q 0%nat := 0 }> [((_ !-> 0%nat), I 2)] [((_ !-> 0%nat), ∣0⟩⟨0∣)].
-Proof.
-Admitted.
+
 
 
 
